Java/src/Java/Logic/SpecLogic.v
@@ -1,4 +1,4 @@
-Require Import Later Program ILogic ILEmbed ILInsts.
+Require Import Later Program ILogic ILEmbed ILInsts Lang RelationClasses.
 
 (*
 Local Existing Instance ILLaterNat.
@@ -11,7 +11,24 @@ Local Existing Instance ILPre_ILogic.
 
 Require Import AssertionLogic.
 
-Definition spec := ILPreFrm Prog_sub (ILPreFrm ge (ILPreFrm extSP Prop)).
+Definition context := list comp_cmd.
+
+Fixpoint cmd_to_context c :=
+  match c with 
+    | cc_seq c1 c2 => (cmd_to_context c1) ++ (cmd_to_context c2)
+    | cc_skip => nil
+    | _ => c::nil
+  end.
+
+Definition ext_cont (c1 c2 : context) := exists c3, c1 = (c2 ++ c3).
+
+Instance ext_cont_Pre: PreOrder ext_cont.
+Proof.
+ split.
+ - exists nil; simpl; rewrite app_nil_r; reflexivity.
+ - intros c1 c2 c3 [c4 H1] [c5 H2]. exists (c5 ++ c4).
+   rewrite H2, <- app_assoc in H1; apply H1.
+Qed.
 
 (*
 Global Instance ILLOperatorsSpec : ILLOperators spec := _.
@@ -20,14 +37,316 @@ Global Instance ILSpec : ILLater spec := _.
 *)
 
 Local Transparent ILPre_Ops.
+Local Transparent ILFun_Ops.
 Require Import Compare_dec.
-Definition mk_spec (f: Program -> nat -> sasn -> Prop)
-  (Hnat: forall k P T, f P (S k) T -> f P k T)
-  (HSPred: forall k P P' T, Prog_sub P P' -> f P k T -> f P' k T)
-  (HSExt: forall k P T U, extSP T U -> f P k T -> f P k U) : spec.
-  refine (mkILPreFrm (fun k => (mkILPreFrm (fun P => (mkILPreFrm (fun T => f k P T)) _)) _) _).
+
+Inductive ST :=
+  | st_end : ST
+  | st_send : var -> sasn -> ST
+  | st_recv : var -> sasn -> ST.
+  
+Inductive label :=
+  | l_tau : label
+  | l_send : channel -> val -> heap -> label
+  | l_recv : channel -> val -> heap -> label
+  | l_start : channel -> comp_cmd -> label.
+  
+Inductive par_context :=
+  | pc_atom : stack -> heap -> context -> par_context
+  | pc_nu : channel -> par_context -> par_context -> par_context.
+  
+Inductive hole_context :=
+  | hc_hole : hole_context
+  | hc_nu1 : channel -> hole_context -> par_context -> hole_context
+  | hc_nu2 : channel -> par_context -> hole_context -> hole_context.
+
+Fixpoint hc_to_pc (hc : hole_context) pc : par_context :=
+	match hc with
+	  | hc_hole => pc
+	  | hc_nu1 a c1 c2 => pc_nu a (hc_to_pc c1 pc) c2
+	  | hc_nu2 a c1 c2 => pc_nu a c1 (hc_to_pc c2 pc)
+	end.
+
+Definition label_channel l :=
+  match l with
+	| l_tau =>  None
+	| l_send c _ _ => Some c
+	| l_recv c _ _ => Some c
+	| l_start c _ => Some c
+  end.
+
+Fixpoint pc_channels (pc : par_context) : list channel :=
+  match pc with
+    | pc_atom _ _ _ => nil
+    | pc_nu c pc1 pc2 => c :: pc_channels pc1 ++ pc_channels pc2
+  end.
+
+Definition wf_par_context pc := NoDup (pc_channels pc).
+ 
+Fixpoint hc_channels (hc : hole_context) : list channel :=
+  match hc with
+    | hc_hole => nil
+    | hc_nu1 c hc pc => c :: hc_channels hc ++ pc_channels pc
+    | hc_nu2 c pc hc => c :: pc_channels pc ++ hc_channels hc
+  end.
+
+Definition list_disjoint {A : Type} (l1 l2 : list A) := 
+	List.Forall (fun a => ~In a l1) l2.
+	
+Lemma list_disjoint_nil (A : Type) (l : list A) :
+	list_disjoint nil l.
 Proof.
-  intros P P' HPP' k. simpl. intros. eapply HSPred. eassumption. assumption.
+  induction l; constructor; [|apply IHl].
+  intros H. inversion H.
+Qed.
+
+Lemma list_disjoint_consI (A : Type) (x : A) (l1 l2 : list A) 
+	(H : list_disjoint l1 l2) (Hx : ~In x l2) :
+	list_disjoint (x::l1) l2.
+Proof.
+  induction H; constructor.
+  + intros H1. 
+    induction H1; subst; [
+      apply Hx; constructor; reflexivity |
+      apply H; apply H1
+    ].
+  + apply IHForall. intros H1. apply Hx.
+  	right; apply H1.
+Qed.
+
+Lemma list_disjoint_sym (A : Type) (l1 l2 : list A)
+	(H : list_disjoint l1 l2) : list_disjoint l2 l1.
+Proof.
+  induction H.
+  + apply list_disjoint_nil.
+  + simpl.
+    apply list_disjoint_consI; assumption.
+Qed.
+
+Lemma list_disjoint_consE (A : Type) (x : A) (l1 l2 : list A) 
+	(H : list_disjoint (x::l1) l2) : 
+	~In x l2 /\ list_disjoint l1 l2.
+Proof.
+  apply list_disjoint_sym in H.
+  inversion H; subst.
+  split; [|apply list_disjoint_sym]; assumption.
+Qed.
+
+Lemma Forall_appE {A : Type} P (l1 l2 : list A)
+	(H : List.Forall P (l1 ++ l2)) : 
+	List.Forall P l1 /\ List.Forall P l2.
+Proof.
+  induction l1; simpl in *.
+  + split; [constructor | assumption].
+  + inversion H; subst.
+    destruct (IHl1 H3) as [H4 H5].
+    split; [constructor|]; assumption.
+Qed.
+
+Lemma Forall_appI {A : Type} P (l1 l2 : list A)
+    (H1 : List.Forall P l1) (H2 : List.Forall P l2) :
+	List.Forall P (l1 ++ l2). 
+Proof.
+  induction l1; simpl in *; [assumption|].
+  inversion H1; subst. constructor; [|apply IHl1]; assumption.
+Qed.
+
+Lemma list_disjoint_appE (A : Type) (l1 l2 l3 : list A) 
+	(H : list_disjoint (l1 ++ l2) l3) :
+	list_disjoint l1 l3 /\ list_disjoint l2 l3.
+Proof.
+  apply list_disjoint_sym in H.
+  apply Forall_appE in H.
+  destruct H as [H1 H2].
+  split; apply list_disjoint_sym; [apply H1|apply H2].
+Qed.
+
+Lemma list_disjoint_appI (A : Type) (l1 l2 l3 : list A) 
+	(H1 : list_disjoint l1 l3) (H2 : list_disjoint l2 l3) :
+	list_disjoint (l1 ++ l2) l3.
+Proof.
+  apply list_disjoint_sym.
+  SearchAbout List.Forall app.
+  apply Forall_appI; apply list_disjoint_sym; [apply H1 | apply H2].
+Qed.
+
+Definition wf_hole_context hc := NoDup (hc_channels hc).
+
+Lemma NoDup_appE {A : Type} (l1 l2 : list A)  (H : NoDup (l1 ++ l2)) :
+	NoDup l1 /\ NoDup l2 /\ list_disjoint l1 l2.
+Proof.
+  induction l1; simpl in *.
+  + repeat split; [constructor | assumption | apply list_disjoint_nil].
+  + inversion H; subst.
+    specialize (IHl1 H3). destruct IHl1 as [Hl1 [Hl2 Hdisj]].
+    repeat split; [|assumption|].
+    * constructor. intros Ha.
+      apply H2. apply in_app_iff; left; assumption.
+      assumption.
+    * apply list_disjoint_consI; [assumption|].
+      intros Ha. apply H2. apply in_app_iff; right; assumption.
+Qed.
+
+Lemma NoDup_appI {A : Type} (l1 l2 : list A) 
+	(Hl1 : NoDup l1) (Hl2 : NoDup l2) (Hdisj : list_disjoint l1 l2) :
+    NoDup (l1 ++ l2).
+Proof.
+  induction l1; simpl in *; [assumption|].
+  inversion Hl1; subst. constructor.
+  + intros H. apply in_app_or in H. destruct H; [apply H1; apply H|].
+    apply list_disjoint_sym in Hdisj. inversion Hdisj; subst.
+    apply H4; apply H.
+  + apply IHl1; [assumption|].
+    apply list_disjoint_sym in Hdisj; inversion Hdisj; subst.
+    apply list_disjoint_sym; apply H4.
+Qed.
+
+Lemma wf_hole_context_nu1E c hc pc 
+	(H : wf_hole_context (hc_nu1 c hc pc)) :
+	wf_hole_context hc /\ wf_par_context pc /\
+	list_disjoint (hc_channels hc) (pc_channels pc) /\
+	~In c (hc_channels hc) /\ ~In c (pc_channels pc).
+Proof.
+  inversion H; subst.
+  apply NoDup_appE in H3 as [H3 [H4 H5]].
+  repeat split; try assumption; intros H1; apply H2;
+  apply in_app_iff; intuition.
+Qed.
+
+Lemma wf_hole_context_nu2E c hc pc 
+	(H : wf_hole_context (hc_nu2 c pc hc)) :
+	wf_hole_context hc /\ wf_par_context pc /\
+	list_disjoint (pc_channels pc) (hc_channels hc) /\
+	~In c (hc_channels hc) /\ ~In c (pc_channels pc).
+Proof.
+  inversion H; subst.
+  apply NoDup_appE in H3 as [H3 [H4 H5]].
+  repeat split; try assumption; intros H1; apply H2;
+  apply in_app_iff; intuition.
+Qed.
+
+Lemma wf_par_context_parI pc1 pc2 c
+	(Hpc1 : wf_par_context pc1) (Hpc2 : wf_par_context pc2)
+	(Hdisj : list_disjoint (pc_channels pc1) (pc_channels pc2)) 
+	(Hc1 : ~In c (pc_channels pc1)) (Hc2 : ~In c (pc_channels pc2)) :
+	wf_par_context (pc_nu c pc1 pc2).
+Proof.
+  unfold wf_par_context in *; simpl.
+  constructor.
+  + intro H; apply in_app_iff in H.
+  	destruct H as [H | H]; [apply Hc1 | apply Hc2]; apply H.
+  + apply NoDup_appI; assumption.
+Qed.
+
+Lemma hc_to_pc_disjoint_channels (hc : hole_context) (pc : par_context) l
+    (H : list_disjoint (hc_channels hc ++ pc_channels pc) l) :
+	list_disjoint (pc_channels (hc_to_pc hc pc)) l.
+Proof.
+  induction hc; simpl in *; intros.
+  + apply H.
+  + rewrite <- app_assoc in H.
+    apply list_disjoint_consE in H as [H H1].
+    apply list_disjoint_appE in H1 as [H1 H2].
+    apply list_disjoint_appE in H2 as [H2 H3].
+    apply list_disjoint_consI; [|assumption].
+    apply list_disjoint_appI; [|assumption].
+    apply IHhc.
+    apply list_disjoint_appI; assumption.
+  + rewrite <- app_assoc in H.
+    apply list_disjoint_consE in H as [H H1].
+    apply list_disjoint_appE in H1 as [H1 H2].
+    apply list_disjoint_appE in H2 as [H2 H3].
+    apply list_disjoint_consI; [|assumption].
+    apply list_disjoint_appI; [assumption|].
+    apply IHhc.
+    apply list_disjoint_appI; assumption.
+Qed.
+
+Lemma hc_to_pc_in c hc pc 
+	(H : In c (pc_channels (hc_to_pc hc pc))) :
+	In c (hc_channels hc) \/ In c (pc_channels pc).
+Proof.
+  induction hc; simpl in *.
+  + right; assumption.
+  + destruct H as [H | H]; subst.
+    * left; left; reflexivity.
+    * apply in_app_or in H as [H | H].
+      specialize (IHhc H). destruct IHhc as [H1 | H1].
+      - left; right; apply in_app_iff; left; assumption.
+      - right; assumption.
+      - left; right; apply in_app_iff; right; assumption.
+  + destruct H as [H | H]; subst.
+    * left; left; reflexivity.
+    * apply in_app_or in H as [H | H].
+      - left; right; apply in_app_iff; left; assumption.
+      - specialize (IHhc H). destruct IHhc as [H1 | H1].
+        left; right; apply in_app_iff; right; assumption.
+        right; assumption.
+Qed.
+
+Lemma wf_hc_to_pc (hc : hole_context) (pc : par_context)
+  (Hhc : wf_hole_context hc) (Hpc : wf_par_context pc)
+  (H : list_disjoint (hc_channels hc) (pc_channels pc)) :
+  wf_par_context (hc_to_pc hc pc).
+Proof.
+  induction hc; simpl in *.
+  + apply Hpc.
+  + pose proof H as H'.
+    apply list_disjoint_consE in H; destruct H as [H H1].
+    apply list_disjoint_appE in H1. destruct H1 as [H1 H2].
+    apply wf_hole_context_nu1E in Hhc.
+    destruct Hhc as [H3 [H4 [H5 [H6 H7]]]].
+	
+    apply wf_par_context_parI.
+    * apply IHhc; assumption.
+    * assumption.
+    * apply hc_to_pc_disjoint_channels.
+      apply list_disjoint_sym in H'; inversion H'; subst.
+      apply list_disjoint_sym in H10. 
+      apply list_disjoint_appE in H10 as [H10 H11].
+      apply list_disjoint_appI.
+      apply H5. apply list_disjoint_sym. apply H11.
+	* intros H8. 
+	  apply hc_to_pc_in in H8; destruct H8 as [H8 | H8].
+	  apply H6; assumption.
+	  apply H; assumption.
+    * assumption.
+  + pose proof H as H'.
+    apply list_disjoint_consE in H; destruct H as [H H1].
+    apply list_disjoint_appE in H1. destruct H1 as [H1 H2].
+    apply wf_hole_context_nu2E in Hhc.
+    destruct Hhc as [H3 [H4 [H5 [H6 H7]]]].
+	
+    apply wf_par_context_parI.
+    * assumption.
+    * apply IHhc; assumption.
+    * apply list_disjoint_sym; 
+      apply hc_to_pc_disjoint_channels.
+      apply list_disjoint_sym in H'; inversion H'; subst.
+      apply list_disjoint_sym in H10. 
+      apply list_disjoint_appE in H10 as [H10 H11].
+      apply list_disjoint_appI.
+      apply list_disjoint_sym.
+      apply H5. apply list_disjoint_sym; apply H10.
+	* assumption.
+	* intros H8.
+	  apply hc_to_pc_in in H8; destruct H8 as [H8 | H8].	
+	  apply H6; assumption.
+	  apply H; assumption.
+Qed.
+
+Definition spec := ILPreFrm Prog_sub (ILPreFrm ge 
+	(Fun context (Fun hole_context (ILPreFrm extSP Prop)))).
+
+Definition mk_spec (f: Program -> nat -> context -> hole_context -> sasn -> Prop)
+  (Hnat: forall k P c hc T, f P (S k) c hc T -> f P k c hc T)
+  (HSPred: forall k P P' c hc T, Prog_sub P P' -> f P k c hc T -> f P' k c hc T)
+  (HSExt: forall k P c hc T U, extSP T U -> f P k c hc T -> f P k c hc U) : spec.
+  refine (mkILPreFrm (fun k => 
+  		   (mkILPreFrm (fun P c hc => 
+  		       (mkILPreFrm (fun T => f k P c hc T) _)) _)) _).
+Proof.
+  intros P P' HPP' k c. simpl. intros. eapply HSPred. eassumption. assumption.
   Grab Existential Variables.
   intros n m Hnk S'. simpl.
    generalize dependent m. induction n; intros.
@@ -36,11 +355,10 @@ Proof.
     * apply IHn. omega. apply Hnat. apply H.
     * subst. apply H.
   + intros; simpl. apply HSExt; assumption.
-
 Defined.
 
 Program Definition prog_spec (X : Program -> Prop) : spec :=
-  mk_spec (fun (P : Program) _ _ => forall (Q : Program) , Prog_sub P Q -> X Q /\ valid_program Q = true) _ _ _.
+  mk_spec (fun (P : Program) _ _ _ _ => forall (Q : Program) , Prog_sub P Q -> X Q /\ valid_program Q = true) _ _ _.
 Next Obligation.
   intros; apply H0; etransitivity; eassumption.
 Qed.
@@ -51,15 +369,114 @@ Local Existing Instance EmbedILPreDropOp.
 Local Existing Instance EmbedILPreDrop.
 Local Existing Instance EmbedOpPropProp.
 Local Existing Instance EmbedPropProp.
-
+(*
 Instance EmbedPropSpecOp : EmbedOp Prop spec := _. 
 Instance EmbedPropSpec : Embed Prop spec := _.
-
+*)
 Definition prog_eq Prog : spec := [prog] (fun P => P = Prog).
 
 Lemma prog_eq_to_prop P (f : Program -> Prop) (H : f P) : prog_eq P |-- [prog] f.
 Proof.
-  intros Q n T HQ R HQR.
+  intros Q n c hc T HQ R HQR.
   specialize (HQ _ HQR).
   simpl in *. subst. intuition congruence.
+Qed.
+
+(* The following code is an adaptation of the coqos code by Jensen, Kennedy and Benton. *)
+
+Require Import BILogic.
+Require Import Model.
+
+Require Import Morphisms.
+
+Program Definition spec_at (G : spec) (R: sasn) :=
+ mk_spec (fun Pr k c hc P => G Pr k c hc (R ** P)) _ _ _.
+Next Obligation.
+ solve_model H.
+Qed.
+Next Obligation.
+ solve_model H0.
+Qed.
+Next Obligation.
+ solve_model H0.
+ destruct H as [V H].
+ exists V. rewrite sepSPA, H; reflexivity.
+Qed.
+
+Infix "@" := spec_at (at level 44, left associativity).
+
+Lemma spec_frame (S : spec) (R : sasn) :
+ S |-- S @ R.
+Proof.
+ intros Pr k c hc P H. unfold spec_at; simpl.
+ assert (extSP P (P ** R)) as HPR by (exists R; reflexivity).
+ rewrite ->sepSPC in HPR. rewrite <-HPR. assumption.
+Qed.
+
+(* For variations of this instance with lentails instead of extSP, look at
+  [spec_at_covar_m] and [spec_at_contra_m]. *)
+  
+Require Import Morphisms.
+
+Instance spec_at_entails_m:
+ Proper (lentails ++> extSP ++> lentails) spec_at.
+Proof.
+ intros S S' HS R R' HR Pr k c hc P H.
+ unfold spec_at in *; simpl in H; simpl.
+ solve_model H; [rewrite <- HR|rewrite <- HS]; reflexivity.
+Qed.
+
+Instance spec_at_equiv_m:
+ Proper (lequiv ++> lequiv ++> lequiv) spec_at.
+Proof.
+ intros S S' HS R R' HR; split; cancel2; (rewrite HS || rewrite HR); reflexivity.
+Qed.
+
+Lemma spec_at_emp S: S @ empSP -|- S.
+Proof.
+ split; [|apply spec_frame].
+ intros Pr k c hc P; unfold spec_at; simpl; rewrite empSPL; intros; assumption.
+Qed.
+
+Lemma spec_at_at S R R': S @ R @ R' -|- S @ (R ** R').
+Proof.
+ split; intros; unfold spec_at; simpl; intros; solve_model H; [
+ 	rewrite sepSPA | rewrite <- sepSPA ]; reflexivity.
+Qed.
+
+Lemma spec_at_forall {T} F R: (Forall x:T, F x) @ R -|- Forall x:T, (F x @ R).
+Proof. split; simpl; intros; apply H. Qed.
+
+Lemma spec_at_exists {T} F R: (Exists x:T, F x) @ R -|- Exists x:T, (F x @ R).
+Proof. split; simpl; intros; apply H. Qed.
+
+Lemma spec_at_true R: ltrue @ R -|- ltrue.
+Proof. split; simpl; intros; apply H. Qed.
+
+Lemma spec_at_false R: lfalse @ R -|- lfalse.
+Proof. split; simpl; intros; apply H. Qed.
+
+Lemma spec_at_and S S' R: (S //\\ S') @ R -|- (S @ R) //\\ (S' @ R).
+Proof. split; simpl; intros; apply H. Qed.
+
+Lemma spec_at_or S S' R: (S \\// S') @ R -|- (S @ R) \\// (S' @ R).
+Proof. split; simpl; intros; apply H. Qed.
+(*
+Lemma spec_at_propimpl p S R: (p ->> S) @ R -|- p ->> (S @ R).
+Proof. 
+  split; simpl; intros. 
+  + specialize (H _ x0 _ x2 _ x4); apply H; [rewrite x6 |assumption]; try reflexivity. 
+  + specialize (H _ x0 _ x2 _ x4). rewrite <- x6. eapply H. reflexivity. assumption.
+Qed.
+*)
+Lemma spec_at_impl S S' R: (S -->> S') @ R -|- (S @ R) -->> (S' @ R).
+Proof.
+ split.
+ - apply limplAdj. rewrite <-spec_at_and.
+   cancel2. apply landAdj. reflexivity.
+ - unfold spec_at; simpl; intros Pr k c hc P H Pr' HPr' k' Hk' P' [Pext HPext] HS.
+   rewrite <- HPext, sepSPA in HS.
+   assert (extSP P (P ** Pext)) by (exists Pext; reflexivity).
+   specialize (H _ HPr' _ Hk' _ H0 HS). rewrite sepSPA in HPext. rewrite HPext in H.
+   assumption.
 Qed.
