Java/src/Java/Semantics/OperationalSemantics.v
@@ -8,67 +8,419 @@ Import SepAlgNotations.
 Set Implicit Arguments.
 Unset Strict Implicit.
 
+
 Section Commands.
 
   Variable (P : Program).
 
-   Inductive sem_cmd : stack -> heap -> cmd -> option (stack * heap * cmd) -> Prop :=
-	| sem_seq_fail s h c1 c2 : sem_cmd s h c1 None -> sem_cmd s h (cseq c1 c2) None
-  	| sem_seq_skip s h c : sem_cmd s h (cseq cskip c) (Some (s, h, c))
-  	| sem_seq_step s h s' h' c1 c1' c2 : 
-  		sem_cmd s h c1 (Some (s', h', c1')) ->
-  		sem_cmd s h (cseq c1 c2) (Some (s', h', cseq c1' c2))
-  		
+  Inductive sem_cmd : stack -> heap -> cmd -> option (stack * heap) -> Prop :=
     | sem_assign s h x v e : 
     	eval e s = v ->
-    	sem_cmd s h (cassign x e) (Some (stack_add x v s, h, cskip))
+    	sem_cmd s h (cassign x e) (Some (stack_add x v s, h))
     
-    | sem_read_fail (ref : ptr) x y f ref (s : stack) (h : heap_ptr) h' :
+    | sem_read_fail (ref : ptr) x y f ref (s : stack) (h : heap_ptr) :
         s y = vptr ref ->
         ~ In (ref, f) h ->
-        sem_cmd s (h, h') (cread x y f) None
+        sem_cmd s h (cread x y f) None
     | sem_read (ref : ptr) x y f ref v (s : stack) (h : heap) :
         s y = vptr ref ->
-        MapsTo (ref, f) v (fst h) ->
-        sem_cmd s h (cread x y f) (Some (stack_add x v s, h, cskip))
+        MapsTo (ref, f) v h ->
+        sem_cmd s h (cread x y f) (Some (stack_add x v s, h))
         
-    | sem_write_fail x f e s h h' ref :
+    | sem_write_fail x f e s h ref :
         s x = vptr ref ->
         ~ In (ref, f) h ->
-        sem_cmd s (h, h') (cwrite x f e) None
-    | sem_write x f e s h h' h'' ref v :
+        sem_cmd s h (cwrite x f e) None
+    | sem_write x f e s h h' ref v :
       s x = vptr ref ->
       In (ref, f) h ->
       eval e s = v ->
       add (ref, f) v h = h' ->
-      sem_cmd s (h, h'') (cwrite x f e) (Some (s, (h', h''), cskip))
-        
-    | sem_alloc x C s s' h h' h'' n fields :
-    	(n, C) <> pnull ->
-    	(forall f, ~ In ((n, C), f) h) ->
-    	field_lookup P C fields ->
-    	sa_mul h
-          (fold_right (fun f h' => add ((n, C), f) (pnull : val) h') heap_ptr_unit fields) h' ->
-    	s' = stack_add x (vptr (n, C)) s ->
-    	sem_cmd s (h, h'') (calloc x C) (Some (s', (h', h''), cskip)).
+      sem_cmd s h (cwrite x f e) (Some (s, h')).
 
-  Inductive run : stack -> heap -> cmd -> nat -> stack -> heap -> Prop :=
-  	| run_skip s h n : run s h cskip n s h
-  	| run_step n s h c s' h' c' s'' h'' : 
-  		sem_cmd s h c (Some (s', h', c')) ->
-  		run s' h' c' n s'' h'' ->
-  		run s h c (S n) s'' h''.
-  
-  Program Definition safe (c : cmd) : spec :=
-  	mk_spec (fun Pr n P => forall s h m, P s h -> n >= m -> exists s' h', run s h c n s' h') _ _ _.
+Require Import Java.Logic.Marshal.
+	Check Marshal.
+
+  Inductive sem_comp_cmd : stack -> heap -> comp_cmd -> context -> option (label * stack * heap * context) -> Prop :=
+    | sem_atom_fail s h c cont : sem_cmd s h c None -> 
+      sem_comp_cmd s h (cc_atom c) cont None
+    | sem_atom s h c cont s' h' : sem_cmd s h c (Some (s', h')) -> 
+      sem_comp_cmd s h (cc_atom c) cont (Some (l_tau, s', h', cont))
+      
+  	| sem_skip s h c : sem_comp_cmd s h cc_skip c (Some (l_tau, s, h, c))
+  	
+  	| sem_send s h a e v hm cont c :
+  	  eval e s = v ->
+  	  s a = vchan c ->
+  	  Marshal P v h hm ->
+  	  sem_comp_cmd s h (cc_send a e) cont (Some (l_send c v hm, s, h, cont))
+  	  
+  	| sem_recv s (h : heap) x a v h hm h'' cont c :
+  	  sa_mul h hm h'' ->
+  	  s a = vchan c ->
+  	  sem_comp_cmd s h (cc_recv x a) cont (Some (l_recv c v hm, stack_add x v s, h'', cont)) 
+  	
+	| sem_seq_fail s h c1 c2 cont : sem_comp_cmd s h c1 (c2::cont) None -> 
+		sem_comp_cmd s h (cc_seq c1 c2) cont None
+  	| sem_seq_step s h s' h' c1 c1' c2 cont l : 
+  		sem_comp_cmd s h c1 (c2::cont) (Some (l, s', h', c1')) ->
+  		sem_comp_cmd s h (cc_seq c1 c2) cont (Some (l, s', h', c1')).
+
+   Inductive sem_par_context : par_context -> label -> par_context -> Prop :=
+     | sem_comp_start s h c ctxt c' s' h' ctxt' v : 
+        sem_comp_cmd s h c ctxt (Some (l_start v c', s', h', ctxt')) -> 
+     	sem_par_context 
+     	  (pc_atom s h (c::ctxt)) l_tau
+     	  (pc_nu v 
+     	      (pc_atom s' h' ctxt) 
+     	  	  (pc_atom (fun _ => null) (empty _) (cmd_to_context c')))
+     | sem_par_send s h c ctxt s' h' h'' ctxt' v a :
+         sem_comp_cmd s h c ctxt (Some (l_send a v h'', s', h', ctxt')) ->
+     	 sem_par_context (pc_atom s h (c::ctxt)) (l_send a v h'') (pc_atom s' h' ctxt')
+     | sem_par_recv s h c ctxt s' h' h'' ctxt' v a :
+         sem_comp_cmd s h c ctxt (Some (l_recv a v h'', s', h', ctxt')) ->
+     	 sem_par_context (pc_atom s h (c::ctxt)) (l_recv a v h'') (pc_atom s' h' ctxt')
+     | sem_par_tau s h c ctxt s' h' ctxt' :
+         sem_comp_cmd s h c ctxt (Some (l_tau, s', h', ctxt')) ->
+     	 sem_par_context (pc_atom s h (c::ctxt)) l_tau (pc_atom s' h' ctxt')
+     | sem_par_par1 p l p' q c :
+         label_channel l <> Some c ->
+         sem_par_context p l p' -> sem_par_context (pc_nu c p q) l (pc_nu c p' q)
+     | sem_par_par2 p l q q' c :
+         label_channel l <> Some c ->
+         sem_par_context q l q' -> sem_par_context (pc_nu c p q) l (pc_nu c p q')
+     | sem_par_comm1 p a v h p' q q' :
+         sem_par_context p (l_send a v h) p' -> 
+         sem_par_context q (l_recv a v h) q' ->
+         sem_par_context (pc_nu a p q) l_tau (pc_nu a p' q')
+     | sem_par_comm2 p a v h p' q q' :
+         sem_par_context p (l_recv a v h) p' -> 
+         sem_par_context q (l_send a v h) q' ->
+         sem_par_context (pc_nu a p q) l_tau (pc_nu a p' q').
+
+  Inductive red : nat -> par_context -> par_context -> Prop := 
+    | red_zero n p : red n p p
+    | red_step n p q r : sem_par_context p l_tau q -> red n q r -> red (S n) p r.
+
+  Lemma red_tau_step n p q (H : sem_par_context p l_tau q) :
+	  exists q, red n p q.
+  Proof.
+    destruct n.
+    + eexists; constructor.
+    + exists q. econstructor; [eassumption | constructor].
+  Qed.
+
+  Lemma sem_par_hc pc l pc' hc (Hsem : sem_par_context pc l pc') 
+    (H : List.Forall (fun c => label_channel l <> Some c) (hc_channels hc)) :
+  	sem_par_context (hc_to_pc hc pc) l (hc_to_pc hc pc').
+  Proof.
+    induction hc; simpl in *.
+    + assumption.
+    + inversion H; subst; clear H.
+      apply Forall_appE in H3 as [H3 _].
+      constructor; [|apply IHhc]; assumption.
+    + inversion H; subst; clear H.
+      apply Forall_appE in H3 as [_ H3].
+      constructor; [|apply IHhc]; assumption.
+  Qed.
+
+  Lemma sem_par_atom s h c ctxt l s' h' ctxt' 
+    (Hl : ~(exists a c, l = l_start a c))
+    (Hsem : sem_comp_cmd s h c ctxt (Some (l, s', h', ctxt'))) :
+  	sem_par_context (pc_atom s h (c::ctxt)) l (pc_atom s' h' ctxt').
+  Proof.
+    destruct l; simpl in *.
+    + constructor; assumption.
+    + constructor; assumption.
+    + constructor; assumption.
+    + exfalso; apply Hl; exists c0, c1; reflexivity.
+  Qed.
+
+  Lemma sem_comp_atom s h c s' h' ctxt
+  	(Hsem : sem_cmd s h c (Some (s', h'))) :
+  	sem_comp_cmd s h (cc_atom c) ctxt (Some (l_tau, s', h', ctxt)).
+  Proof.
+    constructor; assumption.
+  Qed.
+
+End Commands.
+
+  Program Definition safe (c : comp_cmd) : spec :=
+    mk_spec (fun Pr n ctxt hc P => forall s h m, P s h -> n >= m ->
+    	exists pc, red Pr m (hc_to_pc hc (pc_atom s h (cmd_to_context c ++ ctxt))) pc) _ _ _.
   Next Obligation.
-	assert (S k >= m) by omega.
-	destruct (H _ _ _ H0 H2) as [s' [h' HR]].
     admit.
   Qed.
   Next Obligation.
+	destruct H as [R [_ H]].
+	specialize (H _ _ H1).
+	destruct H as [h1 [h2 [HSub [HT HR]]]].
+	specialize (H0 _ _ _ HT H2).
+	destruct H0 as [pc Hred].
+	generalize dependent (cmd_to_context c ++ c0); intros l Hred.
+	induction l.
+	+ simpl in Hred.
+	  destruct m; [admit|].
+	  inversion Hred; subst.
+	  admit.
+	  admit.
+	+ admit.
+ Qed.
+
+Definition has_ST (c : channel) (st : ST) : spec :=
+	mk_spec (fun Pr n ctxt hc P	N	)
+
+
+Print ST.
+Check ST.
+
+
+Definition triple P c Q :=
+	|-- safe cc_skip @ Q -->> safe c @ P.
+
+    Transparent ILPre_Ops.
+    Transparent ILFun_Ops.
+    Require Import IBILogic.
+    Require Import BILInsts.
+    Transparent BILPre_Ops.
+    Transparent BILFun_Ops.
+    
+    Opaque MapSepAlgOps.
+Require Import Model.
+
+
+Lemma write_lemma (x : var) (f : field) (e : dexpr) :
+	@lentails spec _
+	(safe cc_skip @ (`pointsto (x/V) (`f) (eval e)))
+	(safe (cc_atom (cwrite x f e)) @ (Exists v, `pointsto (x/V) (`f) v)).
+Proof.
+  intros Pr k cont hc T Hsafe s h n HT Hkn. 
+  destruct HT as [h1 [h2 [Hord [[v [H1 [H2 [hframe H3]]]] H4]]]].
+  unfold var_expr, liftn, lift in H1, H2, H3; simpl in H1, H2, H3.
+  eapply red_tau_step.  
+  eapply sem_par_hc.
+  eapply sem_par_atom; [intros [a [b H]]; congruence |].
+  eapply sem_comp_atom.
+  eapply sem_write with (ref := val_to_ptr (s x)).
+  destruct (s x); simpl in *; try intuition congruence.
+  eapply (@sa_mul_inL _ _ _ _ _ _ _ _ (val_to_ptr (s x), f)) in H3.
+  destruct H3 as [H3 H5].
+  eapply (@sa_mul_inL _ _ _ _ _ _ _ _ (val_to_ptr (s x), f)) in Hord.
+  intuition congruence.
+  apply H5.
+  admit. reflexivity.
+  reflexivity.
+Qed.
+
+  Lemma test_seq (c1 c2 : comp_cmd) (P Q R : sasn)
+  	(Hc1 : safe cc_skip @ Q |-- safe c1 @ P) 
+  	(Hc2 : safe cc_skip @ R |-- safe c2 @ Q) :
+  	safe cc_skip @ R |-- safe (cc_seq c1 c2) @ P.
+  Proof.
+    
+    Lemma safe_skip S c P (H : S |-- safe c @ P) :
+    	S |-- safe (cc_seq cc_skip c) @ P.
+    Proof.
+      intros Pr k cont hc T Hsafe s h n HT Hkn.
+      simpl in Hkn; simpl. eapply H; eassumption.
+    Qed.
+    
+    Lemma noethu S c1 c2 c3 P Q
+    	(Hc1 : safe c2 @ Q |-- safe c1 @P)
+    	(H : S |-- safe (cc_seq c2 c3) @ Q) :
+    	S |-- safe (cc_seq c1 c3) @ P.
+    Proof.
+      intros Pr k c hc T Hsafe s h n HT Hkn.
+      simpl. rewrite <- app_assoc.
+      specialize (Hc1 Pr k (cmd_to_context c3 ++ c)).
+      eapply Hc1; [|eapply HT | omega].
+      simpl; simpl in H; intros.
+      rewrite app_assoc.
+      eapply H; [eapply Hsafe | eapply H0 | omega].
+	Qed.
+    
+    
+    
+    eapply noethu; [eassumption|].
+    eapply safe_skip. assumption.	
+    Qed.
+      rewrite app_length.
+      Focus 3. omega.
+
+    intros Pr k c T Hsafe s h n HT Hkn.
+    specialize (Hc2 _ _ _ _ Hsafe).
+  	
+	Lemma blurb P c1 c2 : safe @ P @!(cseq c1 c2) |-- safe @ P @! c2.
+	Proof.
+	  intros Pr n cnt Q H s h m HP Hnm. simpl in H.
+	  assert (n + (length (cmd_to_context c1) + length (cmd_to_context c2)) >=
+	  	      m + length (cmd_to_context c1)) as Hnm' by omega.
+	  rewrite app_length in H. 
+	  specialize (H _ _ _ HP Hnm').
+	  destruct H as [s' [h' HRun]].
+      admit.
+    Qed.
+    assert ((safe @ Q @! (cseq c2 cskip)) Pr k c T) by (simpl; rewrite app_nil_r; apply Hc2).
+    apply blurb in H. specialize (Hc1 _ _ _ _ H).
+    simpl in H.
+    simpl in *. specialize (Hc1 s h m 
+    simpl.
+    rewrite blurb.
+	  assert (ext_cont (cmd_to_context c ++ cnt) cont).
+	  	destruct Hcont; subst. simpl in *. rewrite H0.
+	  	exists 
+	  specialize (H _ _ _ _ HP Hnm Hcont).
+	simpl in Hc2.
+
+    Lemma safe_ext (c1 c2 : cmd) :
+    	safe (cseq c1 c2) |-- safe c1.
+    Proof.
+      intros Pr n cnt P H.
+      intros s h m HP Hnm Hcont.
+      
+      assert (safe c1 Pr n (cnt ++ cmd_to_context c2) P -> safe c1 Pr n cnt P).
+      intros. solve_model H0. eexists; reflexivity.
+      apply H0. clear H0. intros s h m HP Hnm Hcont.
+      simpl in H.
+      assert (ext_cont cnt (cmd_to_context c1 ++ cmd_to_context c2)).
+      destruct Hcont.
+	  admit.
+	  admit.
+    Qed.
+    (*
+    Lemma safe_ext (c1 c2 : cmd) :
+    	safe (cseq c1 c2) |-- safe c1.
+    Proof.
+      intros Pr n cnt P H s h m HP Hnm.
+      specialize (H _ _ _ HP Hnm). 
+      destruct H as [cont' [s' [h' [[cont'' Hcont] Hrun]]]].
+      exists (cmd_to_context c2 ++ cont'), s', h'; split; [|rewrite app_assoc; apply Hrun].
+      exists (cmd_to_context c2 ++ cont''). rewrite Hcont. rewrite <- app_assoc. reflexivity.
+    Qed.
+    *)
+    assert ((safe (cseq cskip c2) @ Q) Pr k c T) by (apply Hc2).
+    rewrite safe_ext in H. specialize (Hc1 _ _ _ _ H).
+    specialize (Hc1 _ _ _ HT Hkn).
+    apply Hc1.
+    destruct Hcont. eexists. rewrite H0. simpl.
+    rewrite <- app_assoc. reflexivity.
+    destruct Hc1 as [cont' [s' [h' [Hcont Hrun]]]].
+    unfold ext_cont in Hcont.
+    simpl in Hc2.
+    assert ((Q ** T) s' h') by admit.
+    specialize (Hc2 _ _ _ H0 Hkn).
+    destruct Hc2 as [c'' [s'' [h'' [Hcont2 Hrun2]]]].
+    simpl in Hc2.
+    exists (cmd_to_context c2
+      destruct Hcont as [cont'' Hcont].
+      destruct H as [s' [h' H]]. clear -H.
+      simpl in *. rewrite <- app_assoc in H.
+      
+      generalize dependent c1; generalize dependent c2.
+      induction cnt'; intros; simpl in *.
+      admit.
+      destruct H.
+      destruct Hcnt as [cnt'' Hcnt].
+      rewrite Hcnt in H. simpl in *.
+      specialize (H _ _ _ nil HP Hnm).
+       rewrite <- Hcnt.
+      assert (ext_cont cnt (c2::cnt')) as H1. {
+      	exists (c2::cnt''). rewrite <- Hcnt; reflexivity.
+      }
+      specialize (H _ _ _ _ HP Hnm H1).
+      destruct H as [s' [h' H]]. rewrite <- Hcnt in H.
+      admit.
+    Qed.
+    simpl in Hc2.
+    Lemma test (c1 c2 c3 : cmd) (P Q : sasn) (H : safe c1 @ P |-- safe c2 @ Q) :
+    	safe (cseq c1 c3) @ P |-- safe (cseq c2 c3) @ Q.
+    Proof.
+      intros Pr k c T Hsafe s h n cont HT Hkn Hcont.
+      simpl in Hsafe.
+    specialize 
+      destruct (H s h m).
+      specialize (H _ _ _ _ HP Hnm Hcnt).
+      destruct Hcnt as [cnt'' Hcnt]. rewrite <- Hcnt.
+      destruct H as [s' [h' H]].
+      rewrite <- Hcnt in H. exists s', h'.
+      exists s', h'.
+      destruct Hcnt as [cnt'' Hcnt]. rewrite <- Hcnt.
+      specialize (H _ _ _ _ HP Hnm Hcnt).
+      assert (ext_cont cnt (cnt' ++ (c::nil))). exists (cnt'' ++ (c::nil)).
+      rewrite <- Hcnt. simpl. rewrite app_assoc. reflexivity.
+      specialize (H _ _ _ _ HP Hnm H0).
+      destruct H as [s' [h' H]].
+      exists s', h'.
+      simpl in H.
+      simpl in *.
+    
+    assert (safe c1
+    simpl in Hc1.
+    simpl in Hsafe.
+    simpl in Hc2.
+    simpl in Hc1.
+    specialize (Hc1 _ _ _ _ Hc2).
+  
+  Lemma test_write (x : var) (f : field) (e : dexpr) : 
+    @lentails spec _ 
+    (safe cskip @ (`pointsto x/V `f (eval e)))
+  	((safe (cwrite x f e)) @ (@lexists sasn _ val (fun v => `pointsto x/V `f `v))).
+  Proof.
+    Transparent ILPre_Ops.
+    Transparent ILFun_Ops.
+    intros Pr k c Q HS s h n HQ Hkn.
+    destruct n. admit.
+    destruct HQ as [h1 [h2 [Hsub [[v [H1 H2]] H3]]]].
+    simpl in H1, H2.
+    unfold liftn, lift in H2; simpl in H2.
+    destruct h, h1.
+    unfold var_expr in H1.
+    assert (exists ref, s x = vptr ref) by admit.
+    destruct H as [ref H].
+    simpl in HS.
+    specialize (HS s (h1, h0) (S n)).
+    assert (exists (s' : stack) (h' : heap), run s (h1, h0) cskip (S n) c s' h') by admit.
+    destruct H0 as [s'' [h'' H0]].
+    inversion H0; subst.
+    exists cskip.
+    split; [|constructor].
+    eapply sem_write; try reflexivity; try eassumption.
+    eapply run_step; [|eapply run_skip].
+    eapply sem_write; try reflexivity; try eassumption.
+    simpl in HQ.
+    destruct HQ.
+    exists (cwrite x f e), s, h; constructor.
+    exists cskip, s. destruct h.
+    assert (exists ref, s x = vptr ref) by admit. destruct H as [ref H].
+    exists (add (ref, f) (eval e s) h, h0).
+    eapply run_step; [|eapply run_skip].
+    eapply sem_write; try reflexivity; 
+    try eassumption.
+    constructor.
+    simpl in *.
+    exists cskip, s.
+	destrcut H.
+	simpl in H.
+	assert (S k >= m) by omega.
+	destruct (H _ _ _ H0 H2) as [c' [s' [h' HR]]]; clear H.
+	inversion HR; subst.
+	exists cskip, s', h'. constructor.
+	clear HR.
+	induction c; inversion H3; try congruence; subst.
+	
+	exists cskip, s'0, h'0. constructor.
+    admit.
+  Qed.
+  Next Obligation.
+	unfold extSP in H.
+	destruct H as [R [_ H]].
+	specialize (H _ _ H1). 
 	Require Import BILInsts IBILogic.
 	Transparent SAIBIOps BILFun_Ops.
+	destruct H as [h1 [h2 [Hstar [Hh1 Hh2]]]].
+	assert (k >= k) as Hk by omega.
+	specialize (H0 _ _ _ Hh1 Hk).
+	apply H0.
 	unfold extSP in H.
 	destruct H as [R [_ H]].
 	specialize (H _ _ H1); simpl in H.
